Core/Metatheory/Progress.lean
@@ -1,133 +1,171 @@
-import LeanSubst
 import Core.Term
 import Core.Reduction
 import Core.Typing
 
-import Core.Metatheory.ValueSoundness
+open LeanSubst
 
-theorem progress_lemma :
-  ⊢ G ->
-  Γ = [] ->
-  G&Δ,Γ ⊢ t : T ->
-  Value G t ∨ t = `0 ∨ ∃ t', G ⊢ t ~> t' := by
-intro wf e j
-induction j
-case var => subst e; simp at *
-case global =>
-  subst e
+namespace Core
 
-  sorry
-case mtch =>
-  subst e
-  sorry
-case guard =>
-  subst e
-  sorry
-case lam => apply Or.inl; apply Value.lam
-case lamt => apply Or.inl; apply Value.lamt
-case zero => apply Or.inr; apply Or.inl; rfl
-case refl => apply Or.inl; apply Value.refl
-case app b _ _ _ _ _ _ _ ih1 ih2 =>
-  cases b
-  case _ =>
-    cases ih2 e
-    case _ => sorry
-    case _ => sorry
-  case _ =>
+theorem split_all_or_left : ∀ {n} {A B : Fin n -> Prop}, (∀ i, A i ∨ B i) -> (∀ i, A i) ∨ (∃ i, B i)
+| 0, _, _, _ => Or.inl (Fin.elim0 ·)
+| n + 1, _, _, h =>
+  have h' := λ (i : Fin n) => h i.succ
+  have lem := @split_all_or_left n _ _ h'
+  match lem with
+  | Or.inl lem' =>
+    match h 0 with
+    | Or.inl h2 => Or.inl (Fin.cases h2 lem')
+    | Or.inr h2 => Or.inr ⟨0, h2⟩
+  | Or.inr ⟨k, lem'⟩ => Or.inr ⟨k.succ, lem'⟩
+
+theorem progress : G&Δ,Γ ⊢ t : T -> Γ = [] -> Value G t ∨ ∃ t', G ⊢ t ~> t'
+| .dctor j1 j2 j3 j4 j5, e => Or.inl Value.dctor
+| .mtch (ss := ss) j1 j2 j3 j4 j5, e =>
+  let j1' := λ i => progress (j1 i) e
+  match split_all_or_left j1' with
+  | Or.inl vs =>
     sorry
+  | Or.inr ⟨i, t', r⟩ =>
+    let ss' := Fun.Vec.update ss t' i
+    let r' : G ⊢ ss i ~> ss' i := by subst ss'; simp; exact r
+    Or.inr ⟨_, .match_congr i r' Fun.Vec.update_neq⟩
+| .lam j1 j2, e => Or.inl Value.lam
+| .app j1 j2 j3, e => sorry
+| .lamt j1 j2, e => Or.inl Value.lamt
+| .appt j1 j2 j3, e => sorry
+| .refl j, e => Or.inl Value.refl
+| .cast j1 j2 j3 e1, e2 => sorry
+| .prj j1 j2, e => sorry
+| .allc j1, e => sorry
+| .apptc j1 j2 e1 e2, e3 => sorry
+| .zero j, e => sorry
+| _, _ => sorry
 
-case appt => sorry
-case cast t A _ _ _ _ j _ ih =>
-  cases ih e
-  case _ h =>
-    have lem := refl_is_val j h
-    cases lem;
-    case _ lem =>
-      rcases lem with ⟨e1, e2⟩; subst e1; subst e2
-      apply Or.inr; apply Or.inr; exists t; apply Red.cast
-    case _ lem =>
-      rcases lem with ⟨c1, c2, e⟩; subst e
-      apply Or.inr; apply Or.inr
-      exists (t ▹ c1) `+  (t ▹ c2)
-      apply Red.ctor2_map2; simp; simp
-  case _ lem =>
-     cases lem
-     case _ h => subst h; apply Or.inr; apply Or.inr; exists `0; apply Red.ctor2_absorb2 (v := .cast); simp
-     case _ h =>
-       rcases h with ⟨c', h⟩
-       apply Or.inr; apply Or.inr; exists (t ▹ c')
-       apply Red.ctor2_congr2 (by simp) h
+-- theorem progress_lemma :
+--   ⊢ G ->
+--   Γ = [] ->
+--   G&Δ,Γ ⊢ t : T ->
+--   Value G t ∨ t = `0 ∨ ∃ t', G ⊢ t ~> t' := by
+-- intro wf e j
+-- induction j
+-- case var => subst e; simp at *
+-- case global =>
+--   subst e
 
-case sym ih =>
-  cases ih e
-  case _ ih => sorry
-  case _ ih =>
-    cases ih
-    case _ ih => sorry
-    case _ ih => sorry
+--   sorry
+-- case mtch =>
+--   subst e
+--   sorry
+-- case guard =>
+--   subst e
+--   sorry
+-- case lam => apply Or.inl; apply Value.lam
+-- case lamt => apply Or.inl; apply Value.lamt
+-- case zero => apply Or.inr; apply Or.inl; rfl
+-- case refl => apply Or.inl; apply Value.refl
+-- case app b _ _ _ _ _ _ _ ih1 ih2 =>
+--   cases b
+--   case _ =>
+--     cases ih2 e
+--     case _ => sorry
+--     case _ => sorry
+--   case _ =>
+--     sorry
 
-case seq ih1 ih2 =>
-  cases ih1 e
-  case _ ih1 => sorry
-  case _ ih1 =>
-    cases ih1
-    case _ ih1 => sorry
-    case _ ih1 => sorry
+-- case appt => sorry
+-- case cast t A _ _ _ _ j _ ih =>
+--   cases ih e
+--   case _ h =>
+--     have lem := refl_is_val j h
+--     cases lem;
+--     case _ lem =>
+--       rcases lem with ⟨e1, e2⟩; subst e1; subst e2
+--       apply Or.inr; apply Or.inr; exists t; apply Red.cast
+--     case _ lem =>
+--       rcases lem with ⟨c1, c2, e⟩; subst e
+--       apply Or.inr; apply Or.inr
+--       exists (t ▹ c1) `+  (t ▹ c2)
+--       apply Red.ctor2_map2; simp; simp
+--   case _ lem =>
+--      cases lem
+--      case _ h => subst h; apply Or.inr; apply Or.inr; exists `0; apply Red.ctor2_absorb2 (v := .cast); simp
+--      case _ h =>
+--        rcases h with ⟨c', h⟩
+--        apply Or.inr; apply Or.inr; exists (t ▹ c')
+--        apply Red.ctor2_congr2 (by simp) h
+
+-- case sym ih =>
+--   cases ih e
+--   case _ ih => sorry
+--   case _ ih =>
+--     cases ih
+--     case _ ih => sorry
+--     case _ ih => sorry
+
+-- case seq ih1 ih2 =>
+--   cases ih1 e
+--   case _ ih1 => sorry
+--   case _ ih1 =>
+--     cases ih1
+--     case _ ih1 => sorry
+--     case _ ih1 => sorry
 
 
-case appc ih1 ih2 =>
-  cases ih1 e
-  case _ ih1 => sorry
-  case _ ih1 =>
-    cases ih1
-    case _ ih1 => sorry
-    case _ ih1 => sorry
+-- case appc ih1 ih2 =>
+--   cases ih1 e
+--   case _ ih1 => sorry
+--   case _ ih1 =>
+--     cases ih1
+--     case _ ih1 => sorry
+--     case _ ih1 => sorry
 
-case arrowc ih1 ih2 =>
-  cases ih1 e
-  case _ ih1 => sorry
-  case _ ih1 =>
-    cases ih1
-    case _ ih1 => sorry
-    case _ ih1 => sorry
+-- case arrowc ih1 ih2 =>
+--   cases ih1 e
+--   case _ ih1 => sorry
+--   case _ ih1 =>
+--     cases ih1
+--     case _ ih1 => sorry
+--     case _ ih1 => sorry
 
-case fst ih1 =>
-  cases ih1 e
-  case _ ih1 => sorry
-  case _ ih1 =>
-    cases ih1
-    case _ ih1 => sorry
-    case _ ih1 => sorry
+-- case fst ih1 =>
+--   cases ih1 e
+--   case _ ih1 => sorry
+--   case _ ih1 =>
+--     cases ih1
+--     case _ ih1 => sorry
+--     case _ ih1 => sorry
 
-case snd ih1 =>
-  cases ih1 e
-  case _ ih1 => sorry
-  case _ ih1 =>
-    cases ih1
-    case _ ih1 => sorry
-    case _ ih1 => sorry
+-- case snd ih1 =>
+--   cases ih1 e
+--   case _ ih1 => sorry
+--   case _ ih1 =>
+--     cases ih1
+--     case _ ih1 => sorry
+--     case _ ih1 => sorry
 
-case allc Γ _ ih1 =>
-  have e' : List.map (λ x => x[+1]) Γ = [] := by rw[e]; simp
-  cases ih1 e'
-  case _ ih1 => sorry
-  case _ ih1 =>
-    cases ih1
-    case _ ih1 => sorry
-    case _ ih1 => sorry
+-- case allc Γ _ ih1 =>
+--   have e' : List.map (λ x => x[+1]) Γ = [] := by rw[e]; simp
+--   cases ih1 e'
+--   case _ ih1 => sorry
+--   case _ ih1 =>
+--     cases ih1
+--     case _ ih1 => sorry
+--     case _ ih1 => sorry
 
-case apptc ih1 =>
-  cases ih1 e
-  case _ ih1 => sorry
-  case _ ih1 =>
-    cases ih1
-    case _ ih1 => sorry
-    case _ ih1 => sorry
+-- case apptc ih1 =>
+--   cases ih1 e
+--   case _ ih1 => sorry
+--   case _ ih1 =>
+--     cases ih1
+--     case _ ih1 => sorry
+--     case _ ih1 => sorry
 
-case choice ih1 ih2 =>
-  cases ih1 e
-  case _ ih1 => sorry
-  case _ ih1 =>
-    cases ih1
-    case _ ih1 => sorry
-    case _ ih1 => sorry
+-- case choice ih1 ih2 =>
+--   cases ih1 e
+--   case _ ih1 => sorry
+--   case _ ih1 =>
+--     cases ih1
+--     case _ ih1 => sorry
+--     case _ ih1 => sorry
+
+end Core
