Core/Reduction.lean
@@ -1,2 +1,3 @@
 import Core.Reduction.Definition
 import Core.Reduction.Congr
+import Core.Reduction.Value
